working on speculation support and lazycoin

examples/LazyCoin.v
@@ -4,6 +4,7 @@ Require Import Coq.PArith.PArith.
 Require Import Coq.Program.Equality.
 Require Import Lia.
 Require Import PeanoNat.
+Require Import Classical.
 
 Require Import coqrel.LogicalRelations.
 Require Import models.EffectSignatures.
@@ -21,6 +22,7 @@ Module OneShotLazyCoinImpl.
   Import LinCCALBase.
   Import LTSSpec.
   Import Lang.
+  Import Semantics.
   Import AssertionsSet.
   Import RGILogic.
   Import TPSimulation.
@@ -29,6 +31,7 @@ Module OneShotLazyCoinImpl.
   Import (notations) LinCCAL.
   Import (canonicals) Sig.Plus.
   Open Scope prog_scope.
+  Open Scope rg_relation_scope.
 
   Definition E : layer_interface :=
   {|
@@ -72,25 +75,110 @@ Module OneShotLazyCoinImpl.
             (* racy set implies racy flip *)
         /\  (forall v t w, σ s = Pending v t (set w) ->
               exists ρ π, Δ s ρ π /\ exists b, ρ = Pending b t flip)
-        /\  (exists ρ π, Δ s ρ π).
+        /\  ((forall v w t, σ s <> Pending v t (set w)) -> forall ρ π, Δ s ρ π -> exists b, ρ = Idle b)
+        .
+  
+  Lemma idle_not_pending : forall (u v w : option bool) t, Idle u <> Pending v t (set w).
+  Proof. inversion 1. Qed.
 
-  Definition G t : rg_relation := 
-      fun s1 s2 => forall t', t <> t' ->
-        forall ρ1 π1 ρ2 π2, Δ s1 ρ1 π1 -> Δ s2 ρ2 π2 -> TMap.find t' π1 = TMap.find t' π2.
+  Definition π_independent (P : assertion) := forall s1 s2,
+    σ s1 = σ s2 ->
+    (forall ρ1 π1, Δ s1 ρ1 π1 -> exists ρ2 π2, Δ s2 ρ2 π2 /\ ρ1 = ρ2) ->
+    (forall ρ2 π2, Δ s2 ρ2 π2 -> exists ρ1 π1, Δ s1 ρ1 π1 /\ ρ1 = ρ2) ->
+    P s1 -> P s2.
 
-  Definition R t : rg_relation :=
+  Lemma I_π_independent: π_independent I.
+  Proof.
+    unfold π_independent; intros.
+    unfold I in *. rewrite H in *.
+    destruct H2 as [? ?].
+    split; [|split].
+    - destruct H2.
+      + left.
+        destruct H2.
+        split; auto.
+        intros. specialize (H4 b) as [? [? [? ?]]].
+        specialize (H0 _ _ H4) as [? [? [? ?]]]; subst.
+        eauto.
+      + right.
+        destruct H2 as [b [? [? [? [? ?]]]]].
+        specialize (H0 _ _ H4) as [? [? [? ?]]]; subst.
+        eexists; eauto.
+    - intros.
+      eapply H3 in H4 as [? [? [? ?]]].
+      specialize (H0 _ _ H4) as [? [? [? ?]]]; subst.
+      eauto.
+    - destruct H3. intros.
+      apply H1 in H6 as [? [? [? ?]]]; subst.
+      eapply H4; eauto.
+  Qed.
+  
+
+  Definition domexact_G t : rg_relation := 
+    fun s1 s2 => forall t', t <> t' ->
+        forall ρ1 π1 ρ2 π2, Δ s1 ρ1 π1 -> Δ s2 ρ2 π2 -> TMap.find t' π1 = None <-> TMap.find t' π2 = None.
+  
+  Definition domexact_R t : rg_relation :=
     fun s1 s2 =>
-      forall ρ1 π1 ρ2 π2, Δ s1 ρ1 π1 -> Δ s2 ρ2 π2 -> TMap.find t π1 = TMap.find t π2.
+      forall ρ1 π1 ρ2 π2, Δ s1 ρ1 π1 -> Δ s2 ρ2 π2 -> TMap.find t π1 = None <-> TMap.find t π2 = None.
+  
+  Lemma domexact_RG_compatible : forall t1 t2, t1 <> t2 -> (domexact_G t1 ⊆ domexact_R t2)%RGRelation.
+  Proof.
+    intros. intros ? ?.
+    unfold domexact_R, domexact_G.
+    intros. eapply H0; eauto.
+  Qed.
+
+  Lemma GINV_domexact : forall t1 t2, t1 <> t2 -> (GINV t1 ⊆ domexact_R t2)%RGRelation.
+  Proof.
+    intros. intros ? ?.
+    unfold domexact_R, GINV, Ginv, LiftRelation_Δ.
+    intros.
+    destruct H0 as [? [? [? ?]]].
+    apply H4 in H2.
+    inversion H2; subst.
+    rewrite PositiveMap.gso; auto.
+    eapply (ac_domexact (Δ x)); eauto.
+  Qed.
+
+  Lemma GRET_domexact : forall t1 t2, t1 <> t2 -> (GRET t1 ⊆ domexact_R t2)%RGRelation.
+  Proof.
+    intros. intros ? ?.
+    unfold domexact_R, GRET, Gret, LiftRelation_Δ.
+    intros.
+    destruct H0 as [? [? [? [? ?]]]].
+    apply H4 in H2.
+    inversion H2; subst.
+    rewrite PositiveMap.gro; auto.
+    eapply (ac_domexact (Δ x)); eauto.
+  Qed.
+
+  Lemma domexact_R_refl : forall t s, domexact_R t s s.
+  Proof.
+    intros. intros ? ?.
+    unfold domexact_R, GId.
+    intros; subst.
+    eapply (ac_domexact (Δ s)); eauto.
+  Qed.
+
+  Definition G t : rg_relation := domexact_G t ∩
+    fun s1 s2 => forall t' ls, t <> t' -> ALin t' ls s1 -> ALin t' ls s2.
+
+  Definition R t : rg_relation := domexact_R t ∩
+    fun s1 s2 => forall ls, ALin t ls s1 -> ALin t ls s2.
 
   Lemma Istable {t} : Stable (R t) I I.
   Proof. unfold Stable. apply ConjRightImpl, ImplRefl. Qed.
 
   Lemma ALinstable {t ls}: Stable (R t) I (ALin t ls).
   Proof.
-    unfold Stable, ALin, R.
-    intros ? [[? [? ?]] ?] ? ? ?.
-    rewrite <- H1. auto.
+    unfold Stable, R.
+    intros ? [[? [? [? ?]]] ?] ? ? ?.
+    apply H1 in H. apply H in H3. auto.
   Qed.
+
+  Create HintDb stableDB.
+  Hint Resolve Istable ALinstable : stableDB.
 
   Program Definition Mcoin : layer_implementation E F := {|
     li_impl m :=
@@ -99,4 +187,494 @@ Module OneShotLazyCoinImpl.
       | read => read_impl
       end
   |}.
+  Next Obligation.
+  eapply RGILogic.soundness with (R:=R) (G:=G) (I:=I).
+    (* valid RG *)
+    {
+      constructor.
+      unfold R. intros.
+      destruct H.
+      split; intros.
+      - pose proof ac_nonempty (Δ s) as [? [? ?]].
+        specialize (H2 _ _ H4).
+        specialize (H _ _ _ _ H4 H3).
+        rewrite <- H; auto.
+      - pose proof ac_nonempty (Δ s') as [? [? ?]].
+        specialize (H2 _ _ H4).
+        specialize (H _ _ _ _ H3 H4).
+        rewrite H; auto.
+    }
+    (* G ⊆ R *)
+    {
+      unfold G, R.
+      intros. intros ? ? ?.
+      destruct H0.
+      - destruct H0.
+        eapply domexact_RG_compatible in H0; eauto.
+        split; auto.
+      - do 2 destruct H0.
+        + split; [eapply GINV_domexact|]; eauto.
+          unfold GINV, Ginv, LiftRelation_Δ, ALin in *.
+          destruct H0 as [? [? [? ?]]].
+          intros. apply H2 in H4.
+          inversion H4; subst.
+          rewrite PositiveMap.gso; auto.
+          eapply H3; eauto.
+        + split; [eapply GRET_domexact|]; eauto.
+          unfold GRET, Gret, LiftRelation_Δ, ALin in *.
+          destruct H0 as [? [? [? [? ?]]]].
+          intros. apply H2 in H4.
+          inversion H4; subst.
+          rewrite PositiveMap.gro; auto.
+          eapply H3; eauto.
+        + split; auto.
+          apply domexact_R_refl.
+    }
+    (* method provable *)
+    {
+      intros t.
+      destruct f.
+      (* flip *)
+      {
+        (* precondition *)
+        exists (I //\\ ALin t (Semantics.ls_inv flip)).
+        (* postcondition *)
+        exists (fun ret => I //\\ ALin t (Semantics.ls_linr flip ret)).
+        constructor;
+        try solve_conj_impl;
+        try solve_conj_stable stableDB.
+        {
+          intros ? [? [? [? [? ?]]]].
+          split; auto.
+          - eapply I_π_independent; eauto.
+            intros.
+            exists ρ1. eexists; split; auto.
+            apply H2. constructor; eauto.
+            intros.
+            apply H2 in H3. inversion H3; subst.
+            exists ρ2. eexists; split; eauto.
+          - intros ? ? ?.
+            apply H2 in H3.
+            inversion H3; subst.
+            rewrite PositiveMap.gss; auto.
+        }
+        {
+          intros. intros [? [[? ?] [? [? ?]]]].
+          eapply I_π_independent; eauto.
+          intros. exists ρ1. eexists; split; auto.
+          apply H3. constructor; eauto.
+          intros.
+          apply H3 in H4. inversion H4; subst.
+          do 2 eexists; split; eauto.
+        }
+        {
+          intros.
+          destruct H.
+          unfold ALin in *.
+          eapply H1. eauto.
+        }
+        {
+          simpl; unfold flip_impl.
+          (* perror *)
+          eapply provable_perror with
+            (P' := I //\\ ALin t (ls_inv flip) //\\ fun s => forall v t' w, t <> t' -> σ s <> Pending v t' (set w)).
+          {
+            intros ? ?.
+            destruct (σ s) eqn:eq.
+            - left. split; eauto.
+              rewrite eq. congruence.
+            - destruct op;
+              try (left; split; eauto;
+              rewrite eq; congruence).
+              destruct (Pos.eq_dec t0 t).
+              + left. split; eauto. rewrite eq,e. congruence.
+              + right.
+                destruct H as [[_ ?] ?].
+                apply H in eq as [? [? [? [? ?]]]]; subst.
+                pose proof H1.
+                apply H0 in H1.
+                econstructor; eauto.
+                do 2 econstructor; eauto.
+                econstructor; eauto.
+          }
+          (* set *)
+          eapply provable_vis_safe with
+            (P' := I //\\ ALin t (ls_lini flip))
+            (Q' := fun _ => I //\\ ALin t (ls_linr flip tt));
+          try solve_conj_impl;
+          try solve_conj_stable stableDB.
+          (* no error *)
+          {
+            intros ? [[[_ ?] ?] ?].
+            intros ?.
+            inversion H2; subst.
+            dependent destruction H6.
+            specialize (H1 v t' w H4). auto.
+          }
+          (* inv *)
+          {
+              pupdate_intros_atomic.
+              dependent destruction Hstep0.
+              destruct Hpre as [[? ?] ?].
+              destruct H as [? [? ?]]. simpl in *.
+              specialize (H3 (idle_not_pending _)). clear H2.
+              destruct H.
+              (* two poss *)
+              {
+                destruct H as [? ?].
+                pose proof (H2 true) as [ρt [πt [Hposst ?]]].
+                pose proof (H2 false) as [ρf [πf [Hpossf ?]]].
+                clear H2.
+
+                pose proof H3 _ _ Hposst as [? ?]; subst.
+                pose proof H3 _ _ Hpossf as [? ?]; subst.
+                simpl in *; subst.
+                pose proof H0 _ _ Hposst.
+                pose proof H0 _ _ Hpossf.
+
+                pupdate_start.
+
+                pupdate_trylin_from Hposst.
+                pupdate_forward t0 (InvEv flip).
+                pupdate_finish.
+
+                eapply ACTrylinContinue.
+
+                pupdate_trylin_from Hpossf.
+                pupdate_forward t0 (InvEv flip).
+                pupdate_finish.
+
+                eapply ACTrylinFinish.
+
+                do 2 split.
+                - split; [|split]; simpl; auto.
+                  + left. split; auto. intros.
+                    destruct b;
+                    [ exists (Pending true t0 flip) | exists (Pending false t0 flip) ];
+                    eexists; split; auto;
+                    [ right | left ]; econstructor; eauto;
+                    do 2 constructor; try (do 2 econstructor); auto.
+                  + inversion 1; subst.
+                    do 2 eexists. split.
+                    * left. constructor; eauto.
+                      do 2 constructor; try (do 2 econstructor); auto.
+                    * eauto.
+                  + intros. exfalso. eapply H4. eauto.
+                - unfold ALin; simpl.
+                  inversion 1; subst;
+                  inversion H5; subst;
+                  rewrite PositiveMap.gss; auto.
+                - unfold domexact_G; intros; simpl in *.
+                  do 2 dependent destruction H6;
+                  rewrite PositiveMap.gso; auto;
+                  eapply (ac_domexact Δ1); eauto.
+                - unfold ALin; simpl.
+                  intros.
+                  do 2 dependent destruction H6;
+                  rewrite PositiveMap.gso; auto;
+                  eapply H5; eauto.
+              }
+              (* single poss *)
+              {
+                destruct H as [? [? [ρ [π [Hposs ?]]]]]; subst.
+
+                pose proof H3 _ _ Hposs as [? ?]; subst.
+                pose proof H0 _ _ Hposs.
+                simpl in *.
+
+                pupdate_start.
+
+                pupdate_trylin_from Hposs.
+                pupdate_forward t0 (InvEv flip).
+                pupdate_finish.
+
+                eapply ACTrylinFinish.
+
+                do 2 split.
+                - split; [|split]; simpl; auto.
+                  + right. eexists; split; eauto.
+                    do 2 eexists; split.
+                    constructor; auto.
+                    do 2 constructor; try (do 2 econstructor); auto.
+                    auto.
+                  + inversion 1; subst.
+                    do 2 eexists; split.
+                    constructor; auto.
+                    do 2 constructor; try (do 2 econstructor); auto.
+                    eauto.
+                  + intros. exfalso. eapply H2; eauto.
+                - unfold ALin; simpl.
+                  inversion 1; subst.
+                  rewrite PositiveMap.gss; auto.
+                - unfold domexact_G; intros; simpl in *.
+                  dependent destruction H5.
+                  rewrite PositiveMap.gso; auto;
+                  eapply (ac_domexact Δ1); eauto.
+                - unfold ALin; simpl.
+                  intros.
+                  dependent destruction H5;
+                  rewrite PositiveMap.gso; auto.
+                  eapply H4; eauto.
+              }
+          }
+          (* res *)
+          {
+              pupdate_intros_atomic.
+              dependent destruction Hstep0.
+              destruct Hpre as [[? [? ?]] ?]. simpl in *.
+              clear H1.
+              specialize (H0 _ _ _ eq_refl) as [ρ [π [Hposs [b ?]]]]; subst.
+              pose proof H2 _ _ Hposs.
+
+              pupdate_start.
+
+              pupdate_trylin_from Hposs.
+              pupdate_forward t0 (ResEv flip tt).
+              pupdate_finish.
+
+              eapply ACTrylinContinue.
+
+              pupdate_trylin_from Hposs.
+              pupdate_forward t0 (ResEv flip tt).
+              pupdate_finish.
+
+              eapply ACTrylinFinish.
+
+              Unshelve.
+              2:{ exact true. }
+              2:{ exact false. }
+
+              do 2 split.
+              - split; [|split]; simpl; auto.
+                + left. split; auto. intros.
+                  destruct b0;
+                  [ exists (Idle true) | exists (Idle false) ];
+                  eexists; split; eauto;
+                  [ right | left ];
+                  constructor; eauto;
+                  do 2 constructor; try (do 2 econstructor); auto.
+                + inversion 1.
+                + intros.
+                  do 2 dependent destruction H3; eauto.
+              - unfold ALin; simpl.
+                intros.
+                do 2 dependent destruction H1;
+                rewrite PositiveMap.gss; auto.
+              - unfold domexact_G; intros; simpl in *.
+                do 2 dependent destruction H4;
+                rewrite PositiveMap.gso; auto;
+                eapply (ac_domexact Δ1); eauto.
+              - unfold ALin; simpl.
+                intros.
+                do 2 dependent destruction H4;
+                rewrite PositiveMap.gso; auto;
+                eapply H3; eauto.
+          }
+
+          (* return *)
+          intros.
+          eapply provable_ret_safe; destruct ret;
+          try solve_conj_impl;
+          try solve_conj_stable stableDB;
+          try apply ImplRefl.
+        }
+      }
+      (* read *)
+      {
+        (* precondition *)
+        exists (I //\\ ALin t (Semantics.ls_inv read)).
+        (* postcondition *)
+        exists (fun ret => I //\\ ALin t (Semantics.ls_linr read ret)).
+        constructor;
+        try solve_conj_impl;
+        try solve_conj_stable stableDB.
+        {
+          intros ? [? [? [? [? ?]]]].
+          split; auto.
+          - eapply I_π_independent; eauto.
+            intros.
+            exists ρ1. eexists; split; auto.
+            apply H2. constructor; eauto.
+            intros.
+            apply H2 in H3. inversion H3; subst.
+            exists ρ2. eexists; split; eauto.
+          - intros ? ? ?.
+            apply H2 in H3.
+            inversion H3; subst.
+            rewrite PositiveMap.gss; auto.
+        }
+        {
+          intros. intros [? [[? ?] [? [? ?]]]].
+          eapply I_π_independent; eauto.
+          intros. exists ρ1. eexists; split; auto.
+          apply H3. constructor; eauto.
+          intros.
+          apply H3 in H4. inversion H4; subst.
+          do 2 eexists; split; eauto.
+        }
+        {
+          intros.
+          destruct H.
+          unfold ALin in *.
+          eapply H1. eauto.
+        }
+        {
+          simpl; unfold read_impl.
+          (* loop *)
+          eapply provable_doloop;
+          try solve_conj_impl;
+          try solve_conj_stable stableDB.
+
+          (* get *)
+          eapply provable_vis_safe with
+            (P' := I //\\ ALin t (ls_inv read))
+            (
+              Q' := fun c =>
+                match c with
+                | Some b => I //\\ ALin t (ls_linr read b)
+                | None => I //\\ ALin t (ls_inv read)
+                end
+            );
+          try ((try destruct a); solve_conj_impl);
+          try ((try destruct a); solve_conj_stable stableDB).
+          (* no error *)
+          (* TODO: extract a more general tactic for solving no error *)
+          {
+            apply ImplTauto; intros ? H; destruct σ;
+            inversion H; subst.
+            dependent destruction H5.
+          }
+          (* inv *)
+          {
+            pupdate_intros_atomic.
+            dependent destruction Hstep0.
+            destruct Hpre as [[? [? ?]] ?]; simpl in *.
+
+            pupdate_start.
+            apply ac_steps_refl.
+
+            do 2 split; auto.
+            - split; [|split]; simpl; auto; try inversion 1.
+              intros. eapply H1; eauto.
+              apply idle_not_pending.
+            - unfold domexact_G. simpl. intros.
+              eapply (ac_domexact Δ1); eauto.
+          }
+          (* res *)
+          {
+            intro b.
+            pupdate_intros_atomic.
+            dependent destruction Hstep0.
+            destruct Hpre as [[? [? ?]] ?]; simpl in *.
+            (* clear H1 H0. *)
+            destruct H as [[? ?] | ?]; subst; simpl in *.
+            (* None *)
+            {
+              pupdate_start.
+              apply ac_steps_refl.
+
+              do 2 split; auto.
+              - split; [|split]; simpl; auto; try inversion 1; subst.
+                intros. eapply H1; eauto. inversion 1.
+              - unfold domexact_G. simpl. intros.
+                eapply (ac_domexact Δ1); eauto.
+            }
+            (* Some *)
+            {
+              destruct H as [b0 [? [ρ [π [Hposs ?]]]]]; subst. simpl in *.
+              clear H0.
+              pose proof Hposs.
+              eapply H1 in H as [? ?]; try congruence; subst; simpl in *.
+
+              pupdate_start.
+
+              pupdate_trylin_from Hposs.
+              pupdate_forward t0 (InvEv read).
+              pupdate_forward t0 (ResEv read x).
+              pupdate_finish.
+
+              apply ACTrylinFinish.
+
+              do 2 split.
+              - split; [|split]; simpl; auto.
+                + right. eexists; split; eauto.
+                  exists (Idle x); eexists; split; auto.
+                  econstructor; auto.
+                  apply H2 in Hposs.
+                  eapply rt_trans; do 2 constructor; auto;
+                  try constructor;
+                  [apply step_read_inv | apply step_read_res |].
+                  rewrite PositiveMap.gss; auto.
+                + inversion 1.
+                + intros. dependent destruction H0; eauto.
+              - unfold ALin; simpl.
+                intros. dependent destruction H.
+                rewrite PositiveMap.gss. auto.
+              - unfold domexact_G; simpl.
+                intros. dependent destruction H3.
+                do 2 try rewrite PositiveMap.gso; auto.
+                eapply (ac_domexact Δ1); eauto.
+              - unfold ALin; simpl.
+                intros. dependent destruction H3.
+                do 2 try rewrite PositiveMap.gso; eauto.
+            }
+          }
+
+          destruct ret; 
+          try (eapply provable_ret_safe;
+          try solve_conj_impl;
+          try solve_conj_stable stableDB;
+          try apply ImplRefl).
+
+          (* TODO: get the random value properly *)
+          (* cas *)
+          eapply provable_vis_safe with
+            (P' := I //\\ ALin t (ls_inv read))
+            (Q' := fun (succ : bool) => if succ then I //\\ ALin t (ls_linr read rand) else I //\\ ALin t (ls_inv read));
+          try ((try destruct a); solve_conj_impl);
+          try ((try destruct a); solve_conj_stable stableDB).
+          (* no error *)
+          {
+            apply ImplTauto; intros ? H; destruct σ;
+            inversion H; subst.
+            dependent destruction H5.
+          }
+          (* inv *)
+          {
+            pupdate_intros_atomic.
+            dependent destruction Hstep0.
+            destruct Hpre as [[? [? ?]] ?]; simpl in *.
+
+            pupdate_start.
+            apply ac_steps_refl.
+
+            do 2 split; auto.
+            - split; [|split]; simpl; auto; try inversion 1.
+              intros. eapply H1; eauto.
+              apply idle_not_pending.
+            - unfold domexact_G. simpl. intros.
+              eapply (ac_domexact Δ1); eauto.
+          }
+          (* res *)
+          {
+            intro b.
+            pupdate_intros_atomic.
+            destruct Hpre as [[? [? ?]] ?]; simpl in *.
+            remember (ResEv (cas None (Some rand)) b) as e in Hstep0.
+            inversion Hstep0; subst; try inversion H5; subst.
+            (* succ *)
+            {
+              apply ResEvInversion in H5; subst.
+              
+            }
+            {
+              inversion H4; subst.
+              apply ResEvInversion in H4; subst.
+              
+            }
+          }
+        }
+      }
+    }
+
 End OneShotLazyCoinImpl.
